formalization/DenotationCtx.v
@@ -1,0 +1,32 @@
+From stdpp Require Import mapset.
+From stdpp Require Import natmap.
+From Coq.Program Require Import Wf.
+From CT Require Import CoreLangClass.
+From CT Require Import OperationalSemantics.
+From CT Require Import BasicTypingClass.
+From CT Require Import RefinementTypeClass.
+From CT Require Import Instantiation.
+From CT Require Import Denotation.
+
+Import Atom.
+Import CoreLang.
+Import Tactics.
+Import NamelessTactics.
+Import ListCtx.
+Import OperationalSemantics.
+Import BasicTyping.
+Import BasicTypingProp.
+Import RefinementType.
+Import Qualifier.
+Import Instantiation.
+Import Denotation.
+
+Fixpoint ctxRst (Γ: listctx rty) (p: env -> Prop) :=
+  match Γ with
+  | [] => p ∅
+  | (x, [: b | ϕ]) :: Γ => exists (v: value), ⟦ {: b | ϕ} ⟧ v /\ ctxRst Γ (fun Γv => p (<[x:=v]> Γv))
+  | (x, {: b | ϕ}) :: Γ => forall (v: value), ⟦ {: b | ϕ} ⟧ v -> ctxRst Γ (fun Γv => p (<[x:=v]> Γv))
+  | (x, ρx ⇨ τ) :: Γ => forall (v: value), ⟦ ρx ⇨ τ ⟧ v -> ctxRst Γ (fun Γv => p (<[x:=v]> Γv))
+  end.
+
+Notation "'⟪' Γ '⟫' p " := (ctxRst Γ p) (at level 20, format "⟪ Γ ⟫ p", Γ constr).
